wip

Bridge.fsti
@@ -1,8 +1,6 @@
 module Bridge
 
-module I = FStar.Int
-module UI = FStar.UInt
-module L = FStar.List.Pure
+exception UnReachableError
 
 type result 'a 'b =
 | Ok: v: 'a -> result 'a 'b
@@ -13,12 +11,39 @@ val native_uint_bits: Prims.pos
 
 assume new type native_int
 
-type isize = I.int_t native_int_bits
+type isize = Int.int_t native_int_bits
 
 val of_int: native_int -> Tot isize
 
 val to_native_int:
-    (n:I.int_t native_int_bits)
+    (n:Int.int_t native_int_bits)
     -> Tot (native_n:native_int{of_int native_n = n})
 
-type native_list 'a = (l:list 'a{L.length l <= I.max_int native_int_bits})
+type native_list 'a = (l:list 'a{List.length l <= Int.max_int native_int_bits})
+
+type char = FStar.Char.char
+type ordmap = FStar.OrdMap.ordmap
+
+type native_string = (s:string{List.length (String.list_of_string s) <= Int.max_int native_int_bits})
+
+type native_char = char
+
+assume new type native_map 'k 'v
+
+val empty_native_map: #k:eqtype -> #v:Type -> unit -> Tot (native_map k v)
+val append_native_map: #k:eqtype -> #v:Type -> native_map k v -> k -> v -> Tot (native_map k v)
+
+val dom_select: #k:eqtype -> #v:Type -> #f:OrdMap.cmp k
+    -> (key:k) -> (m:ordmap k v f)
+    -> Lemma
+        (requires OrdSet.mem key (OrdMap.dom m))
+        (ensures Some? (OrdMap.select key m))
+
+let to_native_map (#k:eqtype) (#v:Type) #f (m:ordmap k v f): Tot (native_map k v) =
+    OrdSet.Ext.fold (OrdMap.dom m) (
+        fun key -> fun acc ->
+        (append_native_map #k #v acc key (
+            match OrdMap.select key m with
+                | Some value -> value
+        ))
+    ) (empty_native_map #k #v ())
