nucleotide-count/Nucleotide_count.fst
@@ -1,10 +1,53 @@
 module Nucleotide_count
 open Bridge
-
-open Base
+open List.Lemmas
+module Base = Nucleotide_count.Base
 
 (* Count the number of times a nucleotide occurs in the string. *)
-val count_nucleotide : string -> char -> (int, char) Result.t
+val count_nucleotide: native_string -> native_char
+    -> Tot (result native_int native_char)
+let count_nucleotide data nucleotide =
+    match Base.count_nucleotide data nucleotide with
+    | Ok count -> Ok (to_native_int count)
+    | Error c -> Error c
 
 (* Count the nucleotides in the string. *)
-val count_nucleotides : string -> (int Map.M(Char).t, char) Result.t
+val count_nucleotides: native_string
+    -> Tot (result (native_map native_char native_int) native_char)
+let count_nucleotides data =
+    match Base.count_nucleotides data with
+    | Ok countMap -> Ok (to_native_map (
+        OrdSet.Ext.fold (OrdMap.dom countMap) (
+            fun key -> fun acc ->
+            (OrdMap.update key (
+                assert (forall k. (
+                    match OrdMap.select k (OrdMap.empty #char #pos #Base.cmp_by_code) with
+                        | None -> True
+                ));
+                assert (forall k1 k2 m new_v. (
+                (
+                    match OrdMap.select #_ #_ #Base.cmp_by_code k1 m with
+                    | None -> True
+                    | Some count -> 0 < count /\ count <= Int.max_int native_int_bits
+                ) /\ 0 < new_v /\ new_v <= Int.max_int native_int_bits
+                ==>
+                (
+                    match OrdMap.select k2 (OrdMap.update k1 new_v m) with
+                        | None -> True
+                        | Some count -> 0 < count /\ count <= Int.max_int native_int_bits
+                )));
+                assert (forall k. (
+                    match Base.count_nucleotides data with
+                        | Error _ -> True
+                        | Ok data -> (
+                            match OrdMap.select k data with
+                                | None -> True
+                                | Some count -> 0 < count /\ count <= Int.max_int native_int_bits
+                        )
+                ));
+                match OrdMap.select key countMap with
+                    | Some count -> to_native_int count
+            ) acc)
+        ) (OrdMap.empty #_ #_ #Base.cmp_by_code)
+    ))
+    | Error c -> Error c
