List.Ext.fst
@@ -1,0 +1,9 @@
+module List.Ext
+
+(** [find f l] returns [x] such that [f x] holds. *)
+val find: #a:Type
+        -> f:(a -> Tot bool)
+        -> (l:list a{List.existsb f l})
+        -> Tot (x:a{f x})
+let rec find #a f l = match l with
+  | hd::tl -> if f hd then hd else find f tl
