List.Lemmas.fst
@@ -1,0 +1,53 @@
+module List.Lemmas
+
+module List = FStar.List.Pure
+
+val map2_keep_length:
+                f: ('a1 -> 'a2 -> Tot 'b)
+             -> l1: (list 'a1)
+             -> l2: (list 'a2)
+             -> Lemma (requires (List.length l1 == List.length l2))
+                      (ensures (
+                          List.length (List.map2 f l1 l2)) = List.length l1
+                          /\ (List.length (List.map2 f l1 l2)) = List.length l2)
+                      [SMTPat (List.map2 f l1 l2)]
+let rec map2_keep_length f l1 l2 =
+    match l1, l2 with
+    | [], [] -> ()
+    | x1::xs1, x2::xs2 -> map2_keep_length f xs1 xs2
+
+val zip_keep_length:
+                l1: (list 'a1)
+             -> l2: (list 'a2)
+             -> Lemma (requires (List.length l1 == List.length l2))
+                      (ensures (
+                          List.length (List.zip l1 l2)) = List.length l1
+                          /\ (List.length (List.zip l1 l2)) = List.length l2)
+                      [SMTPat (List.zip l1 l2)]
+let rec zip_keep_length l1 l2 =
+    match l1, l2 with
+    | [], [] -> ()
+    | x1::xs1, x2::xs2 -> zip_keep_length xs1 xs2
+
+val filter_decrease_length:
+                f: ('a -> Tot bool)
+             -> l: (list 'a)
+             -> Lemma (requires True)
+                      (ensures List.length (List.filter f l) <= List.length l)
+                      [SMTPat (List.filter f l)]
+let rec filter_decrease_length f l =
+    match l with
+    | [] -> ()
+    | hd::tl -> filter_decrease_length f tl
+
+val count_decrease_length:
+                #a:eqtype
+             -> x: a
+             -> l: (list a)
+             -> Lemma (requires True)
+                      (ensures List.count x l <= List.length l)
+                      [SMTPat (List.count x l)]
+let rec count_decrease_length x l =
+    match l with
+    | [] -> ()
+    | hd::tl -> count_decrease_length x tl
