OrdSet.Ext.fst
@@ -1,0 +1,20 @@
+module OrdSet.Ext
+module List = FStar.List.Pure
+open FStar.OrdSet
+
+// TODO: Change to lemma of OrdSet.fold (or OrdSetProps.fold ?)
+val fold: #a:eqtype -> #b:Type -> #f:cmp a -> s:ordset a f -> ((key:a{mem key s}) -> b -> Tot b) -> b
+          -> Tot b (decreases (size s))
+let rec fold (#a:eqtype) (#b:Type) #f s g x =
+  if s = empty then x
+  else
+    let Some e = choose s in
+    let a_rest = fold (remove e s) g x in
+    g e a_rest
+
+val insert: #a:eqtype -> #f:cmp a -> a -> ordset a f -> ordset a f
+let insert #_ #_ x s = union s (singleton x)
+
+val as_ordset: #a:eqtype -> #f:cmp a -> list a -> ordset a f
+let as_ordset #a #f l =
+    List.fold_left (fun acc -> fun x -> insert x acc) empty l
