nucleotide-count/Nucleotide_count.Base.fst
@@ -1,0 +1,34 @@
+module Nucleotide_count.Base
+open Bridge
+open List.Lemmas
+module List = FStar.List.Pure
+
+let cmp_by_code (lhs:char) (rhs:char) : bool = Char.int_of_char lhs <= Char.int_of_char rhs
+
+let nucleotide_types = OrdSet.Ext.as_ordset #_ #cmp_by_code ['A'; 'C'; 'G'; 'T']
+
+(* Count the number of times a nucleotide occurs in the string. *)
+val count_nucleotide: string -> char -> Tot (result int char)
+let count_nucleotide data nucleotide =
+    match (String.list_of_string data), nucleotide with
+    | _, nucleotide when not (OrdSet.mem nucleotide nucleotide_types)
+        -> Error nucleotide
+    | data, _ when List.existsb (fun elm -> not (OrdSet.mem elm nucleotide_types)) data
+        -> Error (List.Ext.find (fun elm -> not (OrdSet.mem elm nucleotide_types)) data)
+    | data, nucleotide
+        -> Ok (List.count nucleotide data)
+
+(* Count the nucleotides in the string. *)
+val count_nucleotides: string -> Tot (result (ordmap char pos cmp_by_code) char)
+let count_nucleotides data = match (String.list_of_string data) with
+    | data when List.existsb (fun elm -> not (OrdSet.mem elm nucleotide_types)) data
+        -> Error (List.Ext.find (fun elm -> not (OrdSet.mem elm nucleotide_types)) data)
+    | data
+        -> Ok (
+            OrdSet.fold #_ #(ordmap char pos cmp_by_code) #_ (
+                fun countMap -> fun nucleotide ->
+                    match List.count nucleotide data with
+                        | 0 -> countMap
+                        | count -> OrdMap.update nucleotide count countMap
+            ) (OrdMap.empty) nucleotide_types
+        )
